MartinsConjecture.lean
@@ -35,3 +35,4 @@ import MartinsConjecture.UniformFunctionals
 import MartinsConjecture.ReOperator
 import MartinsConjecture.OperatorLocal
 import MartinsConjecture.ContinuousCase
+import MartinsConjecture.JumpInversion
